Source/DafnyRuntime/DafnyRuntimeDafny/test/dafnyRuntimeTest.dfy
@@ -10,6 +10,9 @@ abstract module DafnyRuntimeTest {
         var a := NativeArray<int>.Make(5);
         for i: size_t := 0 to 5 
             invariant a.Valid()
+            invariant a.Length() == 5
+            invariant fresh(a.Repr)
+            invariant forall j | 0 <= j < i :: a.values[j].Set?
         {
             a.Update(i, i as int);
         }
